%GOLDSTONE
\newpage
\section*{goldstone}

\begin{equation}
  a_p
\equiv
\diagram{
  \node[dot=white,label=above:$p$] (p) at (0,0) {};
  \draw[-<-] (p) to ++(0,-0.5);
}
\hspace{20pt}
  a_p^\dagger
\equiv
\diagram{
  \node[dot=white,label=below:$p$] (p) at (0,0) {};
  \draw[->-] (p) to ++(0,+0.5);
}
\hspace{20pt}
  b_a
\equiv
\diagram{
  \node[dot,label=above:$a$] (a) at (0,0) {};
  \draw[-<-] (a) to ++(0,-0.5);
}
\hspace{20pt}
  b_i
\equiv
\diagram{
  \node[dot,label=above:$i$] (i) at (0,0) {};
  \draw[->-] (i) to ++(0,-0.5);
}
\hspace{20pt}
  b_a^\dagger
\equiv
\diagram{
  \node[dot,label=below:$a$] (a) at (0,0) {};
  \draw[->-] (a) to ++(0,+0.5);
}
\hspace{20pt}
  b_i^\dagger
\equiv
\diagram{
  \node[dot,label=below:$i$] (i) at (0,0) {};
  \draw[-<-] (i) to ++(0,+0.5);
}
\end{equation}

\begin{equation}
  a^{p_1p_2\cdots p_n}_{q_1q_2\cdots q_n}
\equiv
\diagram{
  \node[dot=white] (a1) at (0,0) {};
  \node[dot=white] (a2) at (1,0) {};
  \node (dots) at (1.75,0) {$\cdots$};
  \node[dot=white] (an) at (2.5,0) {};
  \draw (a1)--(a2)--(dots)--(an);
  \draw[->-] (a1) to ++(0,+0.5) node[above] {$p_1$};
  \draw[->-] (a2) to ++(0,+0.5) node[above] {$p_2$};
  \draw[->-] (an) to ++(0,+0.5) node[above] {$p_n$};
  \draw[-<-] (a1) to ++(0,-0.5) node[below] {$q_1$};
  \draw[-<-] (a2) to ++(0,-0.5) node[below] {$q_2$};
  \draw[-<-] (an) to ++(0,-0.5) node[below] {$q_n$};
}
\hspace{20pt}
  \tilde{a}^{p_1p_2\cdots p_n}_{q_1q_2\cdots q_n}
\equiv
\diagram{
  \node[ddot=white] (a1) at (0,0) {};
  \node[ddot=white] (a2) at (1,0) {};
  \node (dots) at (1.75,0) {$\cdots$};
  \node[ddot=white] (an) at (2.5,0) {};
  \draw (a1)--(a2)--(dots)--(an);
  \draw[->-] (a1) to ++(0,+0.5) node[above] {$p_1$};
  \draw[->-] (a2) to ++(0,+0.5) node[above] {$p_2$};
  \draw[->-] (an) to ++(0,+0.5) node[above] {$p_n$};
  \draw[-<-] (a1) to ++(0,-0.5) node[below] {$q_1$};
  \draw[-<-] (a2) to ++(0,-0.5) node[below] {$q_2$};
  \draw[-<-] (an) to ++(0,-0.5) node[below] {$q_n$};
}
\end{equation}

\begin{equation}
  \textstyle(\frac{1}{n!})^2
  v_{p_1p_2\cdots p_n}^{q_1q_2\cdots q_n}
  \tilde{a}^{p_1p_2\cdots p_n}_{q_1q_2\cdots q_n}
\equiv
\diagram{
  \node[draw] (label) at (-0.7,0) {{\mathversion{bold}$v$}};
  \node[ddot=white] (v1) at (0,0) {};
  \node[ddot=white] (v2) at (1,0) {};
  \node (dots) at (1.75,0) {$\cdots$};
  \node[ddot=white] (vn) at (2.5,0) {};
  \draw (label)--(v1)--(v2)--(dots)--(vn);
  \draw[->-] (v1) to ++(0,+0.5);
  \draw[-<-] (v1) to ++(0,-0.5);
  \draw[->-] (v2) to ++(0,+0.5);
  \draw[-<-] (v2) to ++(0,-0.5);
  \draw[->-] (vn) to ++(0,+0.5);
  \draw[-<-] (vn) to ++(0,-0.5);
}
\end{equation}

\begin{equation}
  h_p^qa_q^p
\equiv
\diagram{
  \draw (-0.5,0) node[squarex] (h) {} -- (0,0) node[dot=white] (h1) {}; 
  \draw[->-] (h1) to ++(0,+0.5);
  \draw[-<-] (h1) to ++(0,-0.5);
}
\end{equation}

\begin{equation}
\diagram{
  \draw (-0.5,0) node[squarex] (h) {} -- (0,0) node[dot=white] (h1) {};
  \draw[->-] (h1) to ++(0,+0.5);
  \draw[-<-] (h1) to ++(0,-0.5);
}
=
\diagram{
  \draw (-0.5,0) node[squarex] (h) {} -- (0,0) node[ddot=white] (h1) {};
  \draw[->-] (h1) to ++(0,+0.5);
  \draw[-<-] (h1) to ++(0,-0.5);
}
+
\diagram{
  \draw (-0.5,0) node[squarex] (h) {} -- (0,0) node[ddot=white] (h1) {};
  \draw[-<-] (h1) arc (0:360:-0.25);
}
\end{equation}

\begin{equation}
\diagram{
  \draw (-0.5,0) node[squarex] (h) {} -- (0,0) node[dot=white] (h1) {};
  \draw[->-] (h1) to ++(0,+0.5);
  \draw[-<-] (h1) to ++(0,-0.5);
}
=
\diagram{
  \draw (-0.5,0) node[squarex] (h) {} -- (0,0) node[dot] (h1) {};
  \draw[->-] (h1) to ++(0,+0.5);
  \draw[-<-] (h1) to ++(0,-0.5);
}
+
\diagram{
  \draw (-0.5,0) node[squarex] (h) {} -- (0,0) node[dot] (h1) {};
  \draw[->-] (h1) to ++(-0.25,+0.5);
  \draw[-<-] (h1) to ++(+0.25,+0.5);
}
+
\diagram{
  \draw (-0.5,0) node[squarex] (h) {} -- (0,0) node[dot] (h1) {};
  \draw[->-] (h1) to ++(-0.25,-0.5);
  \draw[-<-] (h1) to ++(+0.25,-0.5);
}
+
\diagram{
  \draw (-0.5,0) node[squarex] (h) {} -- (0,0) node[dot] (h1) {};
  \draw[->-] (h1) to ++(0,-0.5);
  \draw[-<-] (h1) to ++(0,+0.5);
}
\end{equation}

\begin{equation}
  \textstyle\frac{1}{4}\overline{g}_{pq}^{rs}a_{rs}^{pq}
=
\diagram{
  \interaction{2}{g}{(0,0)}{dot=white}{sawtooth};
  \draw[->-] (g1) to ++(0,+0.5);
  \draw[-<-] (g1) to ++(0,-0.5);
  \draw[->-] (g2) to ++(0,+0.5);
  \draw[-<-] (g2) to ++(0,-0.5);
}
\end{equation}

\begin{equation}
\diagram{
  \interaction{2}{g}{(0,0)}{dot=white}{sawtooth};
  \draw[->-] (g1) to ++(0,+0.5);
  \draw[-<-] (g1) to ++(0,-0.5);
  \draw[->-] (g2) to ++(0,+0.5);
  \draw[-<-] (g2) to ++(0,-0.5);
}
=
\diagram{
  \interaction{2}{g}{(0,0)}{ddot=white}{sawtooth};
  \draw[->-] (g1) to ++(0,+0.5);
  \draw[-<-] (g1) to ++(0,-0.5);
  \draw[->-] (g2) to ++(0,+0.5);
  \draw[-<-] (g2) to ++(0,-0.5);
}
+
\diagram{
  \interaction{2}{g}{(0,0)}{ddot=white}{sawtooth};
  \draw[->-] (g1) to ++(0,+0.5);
  \draw[-<-] (g1) to ++(0,-0.5);
  \draw[-<-] (g2) arc (0:360:-0.25);
}
+
\diagram{
  \interaction{2}{g}{(0,0)}{ddot=white}{sawtooth};
  \draw[->-] (g1) arc (0:360:+0.25);
  \draw[-<-] (g2) arc (0:360:-0.25);
}
\end{equation}

\begin{equation}
\diagram{
  \interaction{2}{g}{(0,0)}{dot=white}{sawtooth};
  \draw[->-] (g1) to ++(0,+0.5);
  \draw[-<-] (g1) to ++(0,-0.5);
  \draw[->-] (g2) to ++(0,+0.5);
  \draw[-<-] (g2) to ++(0,-0.5);
}
=
\diagram{
  \interaction{2}{g}{(0,0)}{dot}{sawtooth};
  \draw[->-] (g1) to ++(0,+0.5);
  \draw[-<-] (g1) to ++(0,-0.5);
  \draw[->-] (g2) to ++(0,+0.5);
  \draw[-<-] (g2) to ++(0,-0.5);
}
+
\diagram{
  \interaction{2}{g}{(0,0)}{dot}{sawtooth};
  \draw[->-] (g1) to ++(0,+0.5);
  \draw[-<-] (g1) to ++(0,-0.5);
  \draw[->-] (g2) to ++(-0.25,+0.5);
  \draw[-<-] (g2) to ++(+0.25,+0.5);
}
+
\diagram{
  \interaction{2}{g}{(0,0)}{dot}{sawtooth};
  \draw[->-] (g1) to ++(0,+0.5);
  \draw[-<-] (g1) to ++(0,-0.5);
  \draw[->-] (g2) to ++(-0.25,-0.5);
  \draw[-<-] (g2) to ++(+0.25,-0.5);
}
+
\diagram{
  \interaction{2}{g}{(0,0)}{dot}{sawtooth};
  \draw[->-] (g1) to ++(-0.25,+0.5);
  \draw[-<-] (g1) to ++(+0.25,+0.5);
  \draw[->-] (g2) to ++(-0.25,+0.5);
  \draw[-<-] (g2) to ++(+0.25,+0.5);
}
+
\diagram{
  \interaction{2}{g}{(0,0)}{dot}{sawtooth};
  \draw[->-] (g1) to ++(-0.25,-0.5);
  \draw[-<-] (g1) to ++(+0.25,-0.5);
  \draw[->-] (g2) to ++(-0.25,-0.5);
  \draw[-<-] (g2) to ++(+0.25,-0.5);
}
+
\diagram{
  \interaction{2}{g}{(0,0)}{dot}{sawtooth};
  \draw[->-] (g1) to ++(-0.25,-0.5);
  \draw[-<-] (g1) to ++(+0.25,-0.5);
  \draw[->-] (g2) to ++(-0.25,+0.5);
  \draw[-<-] (g2) to ++(+0.25,+0.5);
}
+
\diagram{
  \interaction{2}{g}{(0,0)}{dot}{sawtooth};
  \draw[->-] (g1) to ++(0,-0.5);
  \draw[-<-] (g1) to ++(0,+0.5);
  \draw[->-] (g2) to ++(-0.25,+0.5);
  \draw[-<-] (g2) to ++(+0.25,+0.5);
}
+
\diagram{
  \interaction{2}{g}{(0,0)}{dot}{sawtooth};
  \draw[->-] (g1) to ++(0,-0.5);
  \draw[-<-] (g1) to ++(0,+0.5);
  \draw[->-] (g2) to ++(-0.25,-0.5);
  \draw[-<-] (g2) to ++(+0.25,-0.5);
}
+
\diagram{
  \interaction{2}{g}{(0,0)}{dot}{sawtooth};
  \draw[->-] (g1) to ++(0,-0.5);
  \draw[-<-] (g1) to ++(0,+0.5);
  \draw[->-] (g2) to ++(0,-0.5);
  \draw[-<-] (g2) to ++(0,+0.5);
}
\end{equation}

\begin{equation}
\diagram{
  \draw (-0.5,0) node[squarex] (h) {} -- (0,0) node[dot=white] (h1) {};
  \draw[->-] (h1) to ++(0,+0.5);
  \draw[-<-] (h1) to ++(0,-0.5);
}
+
\diagram{
  \interaction{2}{g}{(0,0)}{dot=white}{sawtooth};
  \draw[->-] (g1) to ++(0,+0.5);
  \draw[-<-] (g1) to ++(0,-0.5);
  \draw[->-] (g2) to ++(0,+0.5);
  \draw[-<-] (g2) to ++(0,-0.5);
}
=
  E_0
+
\diagram{
  \draw (-0.5,0) node[circlex] (f) {} -- (0,0) node[ddot=white] (f1) {};
  \draw[->-] (f1) to ++(0,+0.5);
  \draw[-<-] (f1) to ++(0,-0.5);
}
+
\diagram{
  \interaction{2}{g}{(0,0)}{ddot=white}{sawtooth};
  \draw[->-] (g1) to ++(0,+0.5);
  \draw[-<-] (g1) to ++(0,-0.5);
  \draw[->-] (g2) to ++(0,+0.5);
  \draw[-<-] (g2) to ++(0,-0.5);
}
\hspace{30pt}
  E_0
\equiv
\diagram{
  \draw (-0.5,0) node[squarex] (h) {} -- (0,0) node[ddot=white] (h1) {};
  \draw[-<-] (h1) arc (0:360:-0.25);
}
+
\diagram{
  \interaction{2}{g}{(0,0)}{ddot=white}{sawtooth};
  \draw[->-] (g1) arc (0:360:+0.25);
  \draw[-<-] (g2) arc (0:360:-0.25);
}
\hspace{30pt}
\diagram{
  \draw (-0.5,0) node[circlex] (f) {} -- (0,0) node[ddot=white] (f1) {};
  \draw[->-] (f1) to ++(0,+0.5);
  \draw[-<-] (f1) to ++(0,-0.5);
}
\equiv
\diagram{
  \draw (-0.5,0) node[squarex] (f) {} -- (0,0) node[ddot=white] (f1) {};
  \draw[->-] (f1) to ++(0,+0.5);
  \draw[-<-] (f1) to ++(0,-0.5);
}
+
\diagram{
  \interaction{2}{g}{(0,0)}{ddot=white}{sawtooth};
  \draw[->-] (g1) arc (0:360:0.25);
  \draw[->-] (g2) to ++(0,+0.5);
  \draw[-<-] (g2) to ++(0,-0.5);
}
\end{equation}

\begin{equation}
\diagram[top, bottom]{
%top
  \node at (0.0,1) {1};
  \node at (0.5,1) {+};
  \draw[overhang] (1.25,1.25) node[ddot] (c1*) {};
  \draw[-<-] (c1*) to ++(-0.25,-0.5);
  \draw[->-] (c1*) to ++(+0.25,-0.5);
%middle
  \draw (-0.5,0) node[circlex](f){} -- (0,0) node[ddot=white](f1){};
  \draw[->-] (f1) to ++(0,+0.5);
  \draw[-<-] (f1) to ++(0,-0.5);
  \node at (0.5,0) {+};
  \interaction{2}{g}{(1,0)}{ddot=white}{sawtooth};
  \draw[->-] (g1) to ++(0,+0.5);
  \draw[-<-] (g1) to ++(0,-0.5);
  \draw[->-] (g2) to ++(0,+0.5);
  \draw[-<-] (g2) to ++(0,-0.5);
%bottom
  \node at (0.0,-1) {1};
  \node at (0.5,-1) {+};
  \draw[overhang] (1.25,-1.25) node[ddot] (c1) {};
  \draw[->-] (c1) to ++(-0.25,+0.5);
  \draw[-<-] (c1) to ++(+0.25,+0.5);
}
=
\diagram{
  \draw (-0.5,+0.5) node[circlex] (f) {} to (0,+0.5) node[ddot] (f1) {};
  \draw[overhang] (0,-0.5) node[ddot] (c1) {};
  \draw[-<-,bend right] (f1) to (c1);
  \draw[->-,bend left ] (f1) to (c1);
}
+
\diagram{
  \draw (-0.5,-0.5) node[circlex] (f) {} to (0,-0.5) node[ddot] (f1) {};
  \draw[overhang] (0,+0.5) node[ddot] (c1*) {};
  \draw[->-,bend left ] (f1) to (c1*);
  \draw[-<-,bend right] (f1) to (c1*);
}
+
\diagram{
  \draw[overhang] (0,+0.5) node[ddot] (c1*) {};
  \draw[overhang] (0,-0.5) node[ddot] (c1)  {};
  \draw[->-=0.25,->-=0.75,bend left ] (c1) to node[midway,ddot] (f1) {} (c1*);
  \draw[-<-,bend right] (c1) to (c1*);
  \draw (f1) to ++(-0.5,0) node[circlex] {};
}
+
\diagram{
  \draw[overhang] (0,+0.5) node[ddot] (c1*) {};
  \draw[overhang] (0,-0.5) node[ddot] (c1)  {};
  \draw[-<-=0.25,-<-=0.75,bend left] (c1) to node[midway,ddot] (f1) {} (c1*);
  \draw[->-,bend right] (c1) to (c1*);
  \draw (f1) to ++(-0.5,0) node[circlex] {};
}
+
\diagram{
  \interaction{2}{g}{(0,0)}{ddot}{sawtooth};
  \draw[overhang] (0,-1) node[ddot] (c1)  {};
  \draw[overhang] (1,+1) node[ddot] (c1*) {};
  \draw[->-,bend left ] (c1) to (g1);
  \draw[-<-,bend right] (c1) to (g1); 
  \draw[->-,bend left ] (g2) to (c1*);
  \draw[-<-,bend right] (g2) to (c1*);
}
\end{equation}

\begin{equation}
\diagram[top, bottom]{
%top
  \draw (-0.5,0.5) node[circlex] (f) {} -- (0,0.5) node[ddot=white] (f1) {};
  \node at (0.5,0.5) {+};
  \interaction{2}{g}{(1,0.5)}{ddot=white}{sawtooth};
  \draw[->-] (f1) to ++(0,+0.5);
  \draw[-<-] (f1) to ++(0,-0.5);
  \draw[->-] (g1) to ++(0,+0.5);
  \draw[-<-] (g1) to ++(0,-0.5);
  \draw[->-] (g2) to ++(0,+0.5);
  \draw[-<-] (g2) to ++(0,-0.5);
%bottom
  \node at (0.5,-0.5) {
    $\exp\left(
    \diagram{
      \interaction{2}{t}{(0,-0.25)}{ddot}{overhang};
      \draw[->-] (t1) to ++(-0.25,+0.5);
      \draw[-<-] (t1) to ++(+0.25,+0.5);
      \draw[->-] (t2) to ++(-0.25,+0.5);
      \draw[-<-] (t2) to ++(+0.25,+0.5);
    }
    \right)$
  };
}
=
\diagram{
  \interaction{2}{g}{(0,+0.5)}{ddot}{sawtooth};
  \interaction{2}{t}{(0,-0.5)}{ddot}{overhang};
  \draw[->-,bend left]  (t1) to (g1);
  \draw[-<-,bend right] (t1) to (g1);
  \draw[->-,bend left]  (t2) to (g2);
  \draw[-<-,bend right] (t2) to (g2);
}
\end{equation}

\begin{equation}
\begin{array}{rl}
\diagram[top, bottom]{
%top
  \node[dot,label=left:{$a$}] (a) at (0.0,1.25) {};
  \node[dot,label=left:{$i$}] (i) at (0.5,1.25) {};
  \node[dot,label=left:{$b$}] (b) at (1.0,1.25) {};
  \node[dot,label=left:{$j$}] (j) at (1.5,1.25) {};
  \draw[-<-] (a) to ++(0,-0.5);
  \draw[->-] (i) to ++(0,-0.5);
  \draw[-<-] (b) to ++(0,-0.5);
  \draw[->-] (j) to ++(0,-0.5);
%mid
  \draw (-0.5,0) node[circlex] (f) {} -- (0,0) node[ddot=white] (f1) {};
  \node at (0.5,0) {+};
  \interaction{2}{g}{(1,0)}{ddot=white}{sawtooth};
  \draw[->-] (f1) to ++(0,+0.5);
  \draw[-<-] (f1) to ++(0,-0.5);
  \draw[->-] (g1) to ++(0,+0.5);
  \draw[-<-] (g1) to ++(0,-0.5);
  \draw[->-] (g2) to ++(0,+0.5);
  \draw[-<-] (g2) to ++(0,-0.5);
%bottom
  \node at (0.5,-1) {
    $\exp\left(
    \diagram{
      \interaction{2}{t}{(0,-0.25)}{ddot}{overhang};
      \draw[->-] (t1) to ++(-0.25,+0.5);
      \draw[-<-] (t1) to ++(+0.25,+0.5);
      \draw[->-] (t2) to ++(-0.25,+0.5);
      \draw[-<-] (t2) to ++(+0.25,+0.5);
    }
    \right)$
  };
}
=&
\diagram{
  \interaction{2}{g}{(0,-0.5)}{ddot}{sawtooth};
  \draw[->-] (g1) to ++(-0.25,1) node[dot,label=left:$a$] {};
  \draw[-<-] (g1) to ++(+0.25,1) node[dot,label=left:$i$] {};
  \draw[->-] (g2) to ++(-0.25,1) node[dot,label=left:$b$] {};
  \draw[-<-] (g2) to ++(+0.25,1) node[dot,label=left:$j$] {};
}
+
\diagram{
  \interaction{2}{t}{(0,-0.5)}{ddot}{overhang};
  \draw[->-=0.25,->-=0.75] (t1) to node[midway,ddot] (f1) {}
    ++(-0.25,1) node[dot,label=left:$a$] {};
  \draw[-<-] (t1) to ++(+0.25,1) node[dot,label=left:$i$] {};
  \draw[->-] (t2) to ++(-0.25,1) node[dot,label=left:$b$] {};
  \draw[-<-] (t2) to ++(+0.25,1) node[dot,label=left:$j$] {};
  \draw (f1) to ++(-0.5,0) node[circlex] {};
}
+
\diagram{
  \interaction{2}{t}{(0,-0.5)}{ddot}{overhang};
  \draw[-<-=0.25,-<-=0.75] (t1) to node[midway,ddot] (f1) {}
    ++(-0.25,1) node[dot,label=left:$i$] {};
  \draw[->-] (t1) to ++(+0.25,1) node[dot,label=left:$a$] {};
  \draw[-<-] (t2) to ++(-0.25,1) node[dot,label=left:$j$] {};
  \draw[->-] (t2) to ++(+0.25,1) node[dot,label=left:$b$] {};
  \draw (f1) to ++(-0.5,0) node[circlex] {};
}
+
\diagram{
  \interaction{2}{t}{(0,-0.5)}{ddot}{overhang};
  \draw[->-=0.25,->-=0.75] (t1) to node[midway,ddot] (g1) {}
    ++(-0.25,1) node[dot,label=left:$a$] {};
  \draw[-<-=0.7] (t1) to ++(+0.25,1) node[dot,label=left:$i$] {};
  \draw[->-=0.25,->-=0.75] (t2) to node[midway,ddot] (g2) {}
    ++(-0.25,1) node[dot,label=left:$b$] {};
  \draw[-<-=0.7] (t2) to ++(+0.25,1) node[dot,label=left:$j$] {};
  \draw[sawtooth] (g1)--(g2);
}
+
\diagram{
  \interaction{2}{t}{(0,-0.5)}{ddot}{overhang};
  \draw[-<-=0.25,-<-=0.75] (t1) to node[midway,ddot] (g1) {}
    ++(-0.25,1) node[dot,label=left:$i$] {};
  \draw[->-=0.7] (t1) to ++(+0.25,1) node[dot,label=left:$a$] {};
  \draw[-<-=0.25,-<-=0.75] (t2) to node[midway,ddot] (g2) {}
    ++(-0.25,1) node[dot,label=left:$j$] {};
  \draw[->-=0.7] (t2) to ++(+0.25,1) node[dot,label=left:$b$] {};
  \draw[sawtooth] (g1)--(g2);
}
\\[-20pt]&
+
\diagram{
  \interaction{2}{t}{(0,-0.5)}{ddot}{overhang};
  \interaction{2}{g}{(1,+0.0)}{ddot}{sawtooth};
  \draw[->-] (t1) to ++(-0.25,1) node[dot,label=left:$a$] {};
  \draw[-<-] (t1) to ++(+0.25,1) node[dot,label=left:$i$] {};
  \draw[->-,bend left] (t2) to (g1);
  \draw[-<-,bend right] (t2) to (g1);
  \draw[->-] (g2) to ++(-0.25,0.5) node[dot,label=left:$b$] {};
  \draw[-<-] (g2) to ++(+0.25,0.5) node[dot,label=left:$j$] {};
}
+
\diagram{
  \interaction{2}{ta}{(0,-0.5)}{ddot}{overhang};
  \interaction{2}{tb}{(2,-0.5)}{ddot}{overhang};
  \interaction{2}{g}{(1,0)}{ddot}{sawtooth};
  \draw[->-=0.7] (ta1) to ++(-0.25,1) node[dot,label=left:$a$] {};
  \draw[-<-=0.3] (ta1) to (g1);
  \draw[->-=0.7] (ta2) to ++(-0.25,1) node[dot,label=left:$b$] {};
  \draw[-<-=0.3] (ta2) to (g2);
  \draw[->-=0.3] (tb1) to (g1);
  \draw[-<-=0.7] (tb1) to ++(+0.25,1) node[dot,label=left:$i$] {};
  \draw[->-=0.3] (tb2) to (g2);
  \draw[-<-=0.7] (tb2) to ++(+0.25,1) node[dot,label=left:$j$] {};
}
+
\diagram{
  \interaction{2}{ta}{(0,-0.5)}{ddot}{overhang};
  \interaction{2}{tb}{(2,-0.5)}{ddot}{overhang};
  \interaction{2}{g}{(1,0.5)}{ddot}{sawtooth};
  \draw[->-] (ta1) to ++(-0.25,1) node[dot,label=left:$a$] {};
  \draw[-<-] (ta1) to ++(+0.25,1) node[dot,label=left:$i$] {};
  \draw[->-,bend left]  (ta2) to (g1);
  \draw[-<-,bend right] (ta2) to (g1);
  \draw[->-,bend left]  (tb1) to (g2);
  \draw[-<-,bend right] (tb1) to (g2);
  \draw[->-] (tb2) to ++(-0.25,1) node[dot,label=left:$b$] {};
  \draw[-<-] (tb2) to ++(+0.25,1) node[dot,label=left:$j$] {};
}
\\[10pt]&
+
\diagram{
  \interaction{2}{ta}{(0,-0.5)}{ddot}{overhang};
  \interaction{2}{tb}{(2,-0.5)}{ddot}{overhang};
  \draw[sawtooth] (0,0) node[ddot] (g1) {} to (1.5,0) node[ddot] (g2) {};
  \draw[->-,bend left]  (ta1) to (g1);
  \draw[-<-,bend right] (ta1) to (g1);
  \draw[->-=0.7] (ta2) to ++(-0.25,1) node[dot,label=left:$a$] {};
  \draw[-<-] (ta2) to (g2);
  \draw[->-] (tb1) to (g2);
  \draw[-<-=0.7] (tb1) to ++(+0.25,1) node[dot,label=left:$i$] {};
  \draw[->-] (tb2) to ++(-0.25,1) node[dot,label=left:$b$] {};
  \draw[-<-] (tb2) to ++(+0.25,1) node[dot,label=left:$j$] {};
}
+
\diagram{
  \interaction{2}{ta}{(0,-0.5)}{ddot}{overhang};
  \interaction{2}{tb}{(2,-0.5)}{ddot}{overhang};
  \draw[sawtooth] (0,0) node[ddot] (g1) {} to (1.5,0) node[ddot] (g2) {};
  \draw[->-,bend left]  (ta1) to (g1);
  \draw[-<-,bend right] (ta1) to (g1);
  \draw[-<-=0.7] (ta2) to ++(-0.25,1) node[dot,label=left:$i$] {};
  \draw[->-] (ta2) to (g2);
  \draw[-<-] (tb1) to (g2);
  \draw[->-=0.7] (tb1) to ++(+0.25,1) node[dot,label=left:$a$] {};
  \draw[-<-] (tb2) to ++(-0.25,1) node[dot,label=left:$j$] {};
  \draw[->-] (tb2) to ++(+0.25,1) node[dot,label=left:$b$] {};
}
+
\diagram{
  \interaction{2}{ta}{(0,-0.5)}{ddot}{overhang};
  \interaction{2}{tb}{(2,-0.5)}{ddot}{overhang};
  \interaction{2}{g}{(0,+0.5)}{ddot}{sawtooth};
  \draw[->-,bend left]  (ta1) to (g1);
  \draw[-<-,bend right] (ta1) to (g1);
  \draw[->-,bend left]  (ta2) to (g2);
  \draw[-<-,bend right] (ta2) to (g2);
  \draw[->-] (tb1) to ++(-0.25,1) node[dot,label=left:$a$] {};
  \draw[-<-] (tb1) to ++(+0.25,1) node[dot,label=left:$i$] {};
  \draw[->-] (tb2) to ++(-0.25,1) node[dot,label=left:$b$] {};
  \draw[-<-] (tb2) to ++(+0.25,1) node[dot,label=left:$j$] {};
}
\end{array}
\end{equation}


\begin{equation}
\diagram{
%top
  \node at (0.0,1) {1};
  \node at (0.5,1) {+};
  \draw[overhang] (1.25,1.25) node[ddot] (c1*) {};
  \draw[-<-] (c1*) to ++(-0.25,-0.5);
  \draw[->-] (c1*) to ++(+0.25,-0.5);
%middle
  \draw (-0.5,0) node[circlex](f){} -- (0,0) node[ddot=white](f1){};
  \draw[->-] (f1) to ++(0,+0.5);
  \draw[-<-] (f1) to ++(0,-0.5);
  \node at (0.5,0) {+};
  \interaction{2}{g}{(1,0)}{ddot=white}{sawtooth};
  \draw[->-] (g1) to ++(0,+0.5);
  \draw[-<-] (g1) to ++(0,-0.5);
  \draw[->-] (g2) to ++(0,+0.5);
  \draw[-<-] (g2) to ++(0,-0.5);
%bottom
  \node at (0.0,-1) {1};
  \node at (0.5,-1) {+};
  \draw[overhang] (1.25,-1.25) node[ddot] (c1) {};
  \draw[->-] (c1) to ++(-0.25,+0.5);
  \draw[-<-] (c1) to ++(+0.25,+0.5);
  \frameit{top, bottom};
%derivative
  \node[framenodes={gray:(tl) (tr) (bl) (br)}] (box) {};
  \draw[overhang] (box.north) node[ddot] (c1deriv) {};
  \draw[->-] (c1deriv) to ++(-0.25,0.5) node[dot,label=left:$a$] {};
  \draw[-<-] (c1deriv) to ++(+0.25,0.5) node[dot,label=left:$i$] {};
}
\end{equation}


\begin{equation}
\diagram{
  \node[dot] (g) at (0,+0.5) {};
  \node[flexdot={4pt}{black}] (c) at (0,-0.5) {};
  \draw[->-] (0,0) [partial ellipse=-90:90:0.25cm and 0.5cm];
  \draw[->-] (0,0) [partial ellipse=-90:90:0.5cm and 0.5cm];
  \draw[->-] (0,0) [partial ellipse=-90:90:-0.25cm and 0.5cm];
  \draw[->-] (0,0) [partial ellipse=-90:90:-0.5cm and 0.5cm];
}
\end{equation}

\begin{equation}
  E^{(2)}
=
\diagram[top,bottom]{
  \node[ddot=white] (g1) at (0,+0.4) {};
  \draw[thick,flexdotted=15 per 1cm] (-0.5,0) to (0.5,0);
  \node[ddot=white] (g2) at (0,-0.4) {};
  \draw[->-] (g1) to ++(-0.25,+0.25);
  \draw[->-] (g1) to ++(+0.25,+0.25);
  \draw[-<-] (g1) to ++(-0.25,-0.25);
  \draw[-<-] (g1) to ++(+0.25,-0.25);
  \draw[->-] (g2) to ++(-0.25,+0.25);
  \draw[->-] (g2) to ++(+0.25,+0.25);
  \draw[-<-] (g2) to ++(-0.25,-0.25);
  \draw[-<-] (g2) to ++(+0.25,-0.25);
}
=
\diagram{
  \node[ddot] (g1) at (0,+0.5) {};
  \draw[thick,flexdotted=15 per 1cm] (-0.7,0) to ++(1.4,0);
  \node[ddot] (g2) at (0,-0.5) {};
  \draw[->-=0.6] (0,0) [partial ellipse=-90:90:-0.5cm and 0.5cm];
  \draw[-<-=0.6] (0,0) [partial ellipse=-90:90:-0.25cm and 0.5cm];
  \draw[->-=0.6] (0,0) [partial ellipse=-90:90:0.25cm and 0.5cm];
  \draw[-<-=0.6] (0,0) [partial ellipse=-90:90:0.5cm and 0.5cm];
}
\end{equation}

\begin{equation}
  E^{(3)}
=
\diagram[top,bottom]{
  \node[ddot=white] (g1) at (0,+0.8) {};
  \draw[thick,flexdotted] (-0.5,+0.4) to ++(1,0);
  \node[ddot=white] (g2) at (0,+0.0) {};
  \draw[thick,flexdotted] (-0.5,-0.4) to ++(1,0);
  \node[ddot=white] (g3) at (0,-0.8) {};
  \draw[->-] (g1) to ++(-0.25,+0.25);
  \draw[->-] (g1) to ++(+0.25,+0.25);
  \draw[-<-] (g1) to ++(-0.25,-0.25);
  \draw[-<-] (g1) to ++(+0.25,-0.25);
  \draw[->-] (g2) to ++(-0.25,+0.25);
  \draw[->-] (g2) to ++(+0.25,+0.25);
  \draw[-<-] (g2) to ++(-0.25,-0.25);
  \draw[-<-] (g2) to ++(+0.25,-0.25);
  \draw[->-] (g3) to ++(-0.25,+0.25);
  \draw[->-] (g3) to ++(+0.25,+0.25);
  \draw[-<-] (g3) to ++(-0.25,-0.25);
  \draw[-<-] (g3) to ++(+0.25,-0.25);
}
=
\diagram{
  \node[ddot] (g1) at (0,+0.8) {};
  \draw[thick,flexdotted] (-1,+0.4) to ++(2,0);
  \node[ddot] (g2) at (0,+0.0) {};
  \draw[thick,flexdotted] (-1,-0.4) to ++(2,0);
  \node[ddot] (g3) at (0,-0.8) {};
  \draw[-<-] (0,0) [partial ellipse=-90:90:-0.8cm and 0.8cm];
  \draw[-<-] (0,0) [partial ellipse=-90:90:+0.8cm and 0.8cm];
  \draw[->-=0.6,bend left =55] (g3) to (g2);
  \draw[->-=0.6,bend right=55] (g3) to (g2);
  \draw[->-=0.6,bend left =55] (g2) to (g1);
  \draw[->-=0.6,bend right=55] (g2) to (g1);
}
+
\diagram{
  \node[ddot] (g1) at (0,+0.8) {};
  \draw[thick,flexdotted] (-1,+0.4) to ++(2,0);
  \node[ddot] (g2) at (0,+0.0) {};
  \draw[thick,flexdotted] (-1,-0.4) to ++(2,0);
  \node[ddot] (g3) at (0,-0.8) {};
  \draw[-<-] (0,0) [partial ellipse=-90:90:-0.8cm and 0.8cm];
  \draw[->-] (0,0) [partial ellipse=-90:90:+0.8cm and 0.8cm];
  \draw[->-=0.6,bend left =55] (g3) to (g2);
  \draw[-<-=0.6,bend right=55] (g3) to (g2);
  \draw[->-=0.6,bend left =55] (g2) to (g1);
  \draw[-<-=0.6,bend right=55] (g2) to (g1);
}
+
\diagram{
  \node[ddot] (g1) at (0,+0.8) {};
  \draw[thick,flexdotted] (-1,+0.4) to ++(2,0);
  \node[ddot] (g2) at (0,+0.0) {};
  \draw[thick,flexdotted] (-1,-0.4) to ++(2,0);
  \node[ddot] (g3) at (0,-0.8) {};
  \draw[->-] (0,0) [partial ellipse=-90:90:-0.8cm and 0.8cm];
  \draw[->-] (0,0) [partial ellipse=-90:90:+0.8cm and 0.8cm];
  \draw[-<-=0.6,bend left =55] (g3) to (g2);
  \draw[-<-=0.6,bend right=55] (g3) to (g2);
  \draw[-<-=0.6,bend left =55] (g2) to (g1);
  \draw[-<-=0.6,bend right=55] (g2) to (g1);
}
\end{equation}

